Fixed #106, generics have arbitrary nesting

src/test/highlight/regression-highlight.dfy
@@ -1,19 +1,27 @@
 // Issue #121: Generic and Regular should be highlighted with the same color
 predicate Generic<Bar>(foo: Bar){}
-predicate Generic<Bar<Foo>>(foo: Bar){}
-predicate Generic<Bar<Foo<Blah>>>(foo: Bar){}
+predicate Generic<Bar<Foo>>(foo: Bar<Foo>){}
+predicate Generic<Bar<Foo<Blah>>>(foo: Bar<Foo<Blah>>){}
+predicate Generic<Bar<Foo<Blah<P>>>>(foo: Bar<Foo<Blah<P>>>){}
 predicate Regular(foo: Baz){}
+
+function test() {
+  purple("hello")
+       //^^^^^^^ should be a string
+}
 
 // Issue#120: 'Purple?' should be highlighted entirely
 predicate Purple?(foo: Bar){}
 predicate IsPurple(foo: Bar){}
 
-// NOT WORKING YET - need semantic highlighting
 // Issue#106: The three "bool" should be blue
-datatype D = D((bool) -> bool) | E(bool)
+datatype D = D((bool, int) -> bool) | E(bool)
 
 // Issue#85: Strings should be highlighted correctly.
-method Foo() returns (res: Result<string, string>)
+method {:extern "foo"} Foo() returns (res: Result<string, string>)
+      // ^^^^^^ attribute
+ensures {:verify false} doSomething(res)
+              // ^^^^^ keyword
   {
     :- Need(true, "Not a string, the parens are doing it ().");
     :- Need(!false, @"The code is highlighted as a string
@@ -25,25 +33,46 @@ method Foo() returns (res: Result<string, string>)
 //           Bar should be a function
 function Foo1(bar: string): string {
   Bar<string>(bar)
+  //  ^^^^^^ should be a highlighted keyword 
 }
 
 // Issue#79-1: `Foo2` should be a function
 // Issue#79-2: `Bar` should be a function
 function Foo2<T>(bar: T): T {
-  Bar<Boxed<T>>(Box(arg)).value
+  Bar<Boxed<T>>(Box<T>(arg)).value
+  //  ^^^^^ should be highlighted as a type
+              //^^^ ^ method call + type
 }
 // Issue#79-3: `Bar` should be a function
 function Bar<T>(arg: T): T {
+         //  ^       ^   ^   should be a type
   arg
 }
+
 datatype Boxed<T> = Box(value: T)
+//^^^^^^ keyword
+//       ^^^^^ type
+//             ^ type
+
+datatype MyThing = MyThingConstructor
+//                 ^^^^^^^^^^^^^^^^^^ ideally like a method, but needs semantics
 
 method test() {
 // Issue#70 The string should be highlighted correctly
   var tmp := "This string does not have any reserved words that should be highlighted.";
 }
+class {:extern "MyClass"} MyClass<T, U, V> {
+}                      // ^^^^^^^ ^  ^  ^  should be a type
 
-class {:extern} MyClass<T, U, V> {}
+class MyClass2<T, U, V> {
+}  // ^^^^^^^^ ^  ^  ^  should be a type
+
+class MyClass3 {
+}  // ^^^^^^^^ should be a type
+
+class {:extern "MyClass3"} MyClass3 {
+}                       // ^^^^^^^^ should be a type
+
 
 method MyMethod(x: MyClass<bool, int, bool>, k: int)
 // Text#68         ^^^^^^^ ^^^^  ^^^  ^^^^ should all be blue   
@@ -51,7 +80,8 @@ method MyMethod(x: MyClass<bool, int, bool>, k: int)
 // Issue#64-1: This comment should be highlighted as a comment
 class Foo
   // Issue#64-2: This comment should be highlighted as a comment
-  extends Bar
+  extends Bar<T>
+//^^^^^^^ ^^^ should be highlighted as keywords and type
 {}
 
 method CallGeneral() {
